Coq/src/PermSort.v
@@ -1,0 +1,61 @@
+Require Import Thesis.Free.
+Require Import Thesis.Base.
+Require Import Thesis.Effect.
+Require Import Thesis.Handler.
+Require Import Lists.List.
+
+Import ListNotations.
+
+Section PermSort.
+  Fixpoint insert' fx xs : Prog (List nat) :=
+    match xs with
+    | Nil' _ => Fail
+    | Cons' fy fys => consM fy ((consM fx fys) ? (fys >>= insert' fx))
+    end.
+  
+  Definition insert (fx : Prog nat) (fxs : Prog (List nat)) : Prog (List nat) :=
+    Share fx >>= fun fx' => (consM fx' fxs) ? (fxs >>= insert' fx').
+
+  Fixpoint perm' (xs : List nat) : Prog (List nat) :=
+    match xs with
+    | Nil' _ => nilM
+    | Cons' mx mxs => mxs >>= fun mxs' => insert mx (perm' mxs')
+    end.
+
+  Definition perm (mxs : Prog (List nat)) : Prog (List nat) :=
+    mxs >>= perm'.
+
+  Fixpoint isSorted'' (mx : Prog nat) (xs : List nat) : Prog bool :=
+    match xs with
+    | Nil' _ => pure true
+    | Cons' my mys => mx >>= fun x => my >>= fun y =>
+                       if Nat.leb x y
+                         then mys >>= fun ys => isSorted'' (pure y) ys
+                         else pure false
+    end.
+
+  Fixpoint isSorted' (mx : Prog nat) (mxs : Prog (List nat)) : Prog bool :=
+    mxs >>= fun xs => isSorted'' mx xs.
+
+  Definition isSorted (mxs : Prog (List nat)) : Prog bool :=
+    mxs >>= fun xs => match xs with
+                   | Nil' _ => pure true
+                   | Cons' my mys => isSorted' my mys
+                   end.
+  
+  Definition sort (l : Prog (List nat)) : Prog (List nat) :=
+    Share (perm l) >>= fun xs => isSorted xs >>= fun b => if b then xs else Fail.
+  
+  Inductive sorted : List nat -> Prop :=
+  | sort_nil  : sorted (Nil' nat)
+  | sort_singleton : forall n, sorted (Cons' (pure n) nilM)
+  | sort_cons : forall n m ns, le n m -> sorted (Cons' (pure n) (consM (pure m) ns)).
+
+  Inductive singleton {A} : list A -> Prop :=
+  | singletn : forall (x : A), singleton [x].
+
+  Definition testList := convert [5;42;3;1].
+
+  Lemma sorted_testList : let xs := handle (sort testList) in Forall sorted xs /\ singleton xs.
+    Proof. repeat econstructor. Qed.
+End PermSort.
